Update Binary_operations.thy

Binary_operations.thy
@@ -1,36 +1,150 @@
+
 theory Binary_operations
-  imports Bij_betw_simplicial_complex_bool_func
+ imports Bij_betw_simplicial_complex_bool_func
 begin
 
-definition bool_fun_or :: "(bool^'n \<Rightarrow> bool) \<Rightarrow> (bool^'n \<Rightarrow> bool) \<Rightarrow> (bool^'n \<Rightarrow> bool)"
+definition bool_fun_or :: "nat \<Rightarrow> (bool vec \<Rightarrow> bool) \<Rightarrow> (bool vec \<Rightarrow> bool) \<Rightarrow> (bool vec \<Rightarrow> bool)"
+  where "(bool_fun_or n f g) \<equiv> (\<lambda>x. f x \<or> g x)"
+
+definition bool_fun_and :: "nat \<Rightarrow> (bool vec \<Rightarrow> bool) \<Rightarrow> (bool vec \<Rightarrow> bool) \<Rightarrow> (bool vec \<Rightarrow> bool)"
+  where "(bool_fun_and n f g) \<equiv> (\<lambda>x. f x \<and> g x)"
+
+
+(*definition bool_fun_or :: "(bool^'n \<Rightarrow> bool) \<Rightarrow> (bool^'n \<Rightarrow> bool) \<Rightarrow> (bool^'n \<Rightarrow> bool)"
   where "(bool_fun_or f g) x \<equiv> (f x) \<or> (g x)"
 
 definition bool_fun_and :: "(bool^'n \<Rightarrow> bool) \<Rightarrow> (bool^'n \<Rightarrow> bool) \<Rightarrow> (bool^'n \<Rightarrow> bool)"
   where "(bool_fun_and f g) x \<equiv> (f x) \<and> (g x)"
 
-definition bool_fun_ast :: "(bool^'n \<Rightarrow> bool) \<Rightarrow> (bool^'m \<Rightarrow> bool) \<Rightarrow> ((bool^'n) \<Rightarrow>(bool^'m) \<Rightarrow> bool)"
+definition bool_fun_ast :: "(bool^'n \<Rightarrow> bool) \<Rightarrow> (bool^'m \<Rightarrow> bool) \<Rightarrow> (bool^('n+'m) \<Rightarrow> bool)"
   where "(bool_fun_ast f g) x y \<equiv> (f x) \<and> (g y)"
 
+definition set_ast :: "('a set) \<Rightarrow> ('a set) \<Rightarrow> ('a set)"
+  where "set_ast A B = {}"*)
+
+lemma eq_union_or: 
+  "simplicial_complex_induced_by_monotone_boolean_function n (bool_fun_or n f g)
+  = simplicial_complex_induced_by_monotone_boolean_function n f \<union> simplicial_complex_induced_by_monotone_boolean_function n g"
+  (is "?sc n (?bf_or n f g) = ?sc n f \<union> ?sc n g")
+proof
+  show "?sc n f \<union> ?sc n g \<subseteq> ?sc n (?bf_or n f g)"
+  proof
+    fix \<sigma> :: "nat set"
+    assume "\<sigma> \<in> (?sc n f \<union> ?sc n g)"
+    hence sigma: "\<sigma> \<in> ?sc n f \<or> \<sigma> \<in> ?sc n g" by auto
+    have "f (simplicial_complex.bool_vec_from_simplice n \<sigma>) 
+           \<or> g (simplicial_complex.bool_vec_from_simplice n \<sigma>)"
+    proof (cases "\<sigma> \<in> ?sc n f")
+      case True
+      from simplicial_complex.simplicial_complex_implies_true [OF True]
+      show "f (simplicial_complex.bool_vec_from_simplice n \<sigma>) 
+           \<or> g (simplicial_complex.bool_vec_from_simplice n \<sigma>)" by fast
+    next
+      case False
+      hence sigmain: "\<sigma> \<in> ?sc n g" using sigma by fast
+      from simplicial_complex.simplicial_complex_implies_true [OF sigmain]
+      show "f (simplicial_complex.bool_vec_from_simplice n \<sigma>) 
+           \<or> g (simplicial_complex.bool_vec_from_simplice n \<sigma>)" by fast
+    qed
+    thus "\<sigma> \<in> ?sc n (?bf_or n f g)"
+      using simplicial_complex_induced_by_monotone_boolean_function_def
+      using bool_fun_or_def sigma by auto
+  qed
+next
+  show "?sc n (?bf_or n f g) \<subseteq> ?sc n f \<union> ?sc n g"
+  proof
+    fix \<sigma>::"nat set"
+    assume sigma: "\<sigma> \<in> ?sc n (?bf_or n f g)"
+    hence "bool_fun_or n f g (simplicial_complex.bool_vec_from_simplice n \<sigma>)"
+      unfolding simplicial_complex.bool_vec_from_simplice_def
+      unfolding simplicial_complex_induced_by_monotone_boolean_function_def
+      unfolding ceros_of_boolean_input_def
+      by auto (smt (verit) dim_vec eq_vecI index_vec)+
+    hence "(f (simplicial_complex.bool_vec_from_simplice n \<sigma>)) \<or> (g (simplicial_complex.bool_vec_from_simplice n \<sigma>))"
+      unfolding bool_fun_or_def
+      by auto
+    hence "\<sigma> \<in> ?sc n f \<or> \<sigma> \<in> ?sc n g"
+      by (smt (z3) sigma bool_fun_or_def mem_Collect_eq simplicial_complex_induced_by_monotone_boolean_function_def)
+    thus "\<sigma> \<in> simplicial_complex_induced_by_monotone_boolean_function n f \<union> simplicial_complex_induced_by_monotone_boolean_function n g"
+      by auto
+  qed
+qed
+
+lemma eq_inter_and:
+  "simplicial_complex_induced_by_monotone_boolean_function n (bool_fun_and n f g)
+  = simplicial_complex_induced_by_monotone_boolean_function n f \<inter> simplicial_complex_induced_by_monotone_boolean_function n g"
+  (is "?sc n (?bf_and n f g) = ?sc n f \<inter> ?sc n g")
+proof
+  show "?sc n f \<inter> ?sc n g \<subseteq> ?sc n (?bf_and n f g)"
+  proof
+    fix \<sigma> :: "nat set"
+    assume "\<sigma> \<in> (?sc n f \<inter> ?sc n g)"
+    hence sigma: "\<sigma> \<in> ?sc n f \<and> \<sigma> \<in> ?sc n g" by auto
+    have "f (simplicial_complex.bool_vec_from_simplice n \<sigma>) 
+           \<and> g (simplicial_complex.bool_vec_from_simplice n \<sigma>)"
+    proof -
+      from sigma have sigmaf: "\<sigma> \<in> ?sc n f" and sigmag: "\<sigma> \<in> ?sc n g"
+        by auto
+      have "f (simplicial_complex.bool_vec_from_simplice n \<sigma>)"
+        using simplicial_complex.simplicial_complex_implies_true [OF sigmaf] .
+      moreover have "g (simplicial_complex.bool_vec_from_simplice n \<sigma>)"
+        using simplicial_complex.simplicial_complex_implies_true [OF sigmag] .
+      ultimately show ?thesis by fast
+    qed
+    thus "\<sigma> \<in> ?sc n (?bf_and n f g)"
+      unfolding simplicial_complex_induced_by_monotone_boolean_function_def
+      unfolding bool_fun_and_def
+      using sigma apply auto
+      by (smt (z3) Collect_cong ceros_of_boolean_input_def dim_vec index_vec mem_Collect_eq 
+          simplicial_complex.bool_vec_from_simplice_def 
+          simplicial_complex_induced_by_monotone_boolean_function_def)
+  qed
+next
+  show "?sc n (?bf_and n f g) \<subseteq> ?sc n f \<inter> ?sc n g"
+  proof
+    fix \<sigma> :: "nat set"
+    assume sigma: "\<sigma> \<in> ?sc n (?bf_and n f g)"
+    hence "bool_fun_and n f g (simplicial_complex.bool_vec_from_simplice n \<sigma>)"
+      unfolding simplicial_complex.bool_vec_from_simplice_def
+      unfolding simplicial_complex_induced_by_monotone_boolean_function_def
+      unfolding ceros_of_boolean_input_def
+      by auto (smt (verit) dim_vec eq_vecI index_vec)+
+    hence "(f (simplicial_complex.bool_vec_from_simplice n \<sigma>)) \<and> (g (simplicial_complex.bool_vec_from_simplice n \<sigma>))"
+      unfolding bool_fun_and_def
+      by auto
+    hence "\<sigma> \<in> ?sc n f \<and> \<sigma> \<in> ?sc n g"
+      using bool_fun_and_def sigma simplicial_complex_induced_by_monotone_boolean_function_def by auto
+    thus "\<sigma> \<in> simplicial_complex_induced_by_monotone_boolean_function n f \<inter> simplicial_complex_induced_by_monotone_boolean_function n g"
+      by auto
+  qed
+qed
+
+definition bool_fun_ast :: "(nat \<times> nat) \<Rightarrow> (bool vec \<Rightarrow> bool) \<times> (bool vec \<Rightarrow> bool) \<Rightarrow> (bool vec \<times> bool vec \<Rightarrow> bool)"
+  where "(bool_fun_ast n f) \<equiv> (\<lambda> (x,y). (fst f x) \<and> (snd f y))"
+
 definition
-  simplicial_complex_induced_by_monotone_boolean_function_ast 
-    :: "(bool^'n::class_mod_type => bool^'m::class_mod_type \<Rightarrow> bool) => ('n set * 'm set) set"
-  where "simplicial_complex_induced_by_monotone_boolean_function_ast f = 
-        {z. \<exists>x y. f x y \<and> ((ceros_of_boolean_input x), (ceros_of_boolean_input y)) = z}"
+  simplicial_complex_induced_by_monotone_boolean_function_ast
+    :: "(nat \<times> nat) \<Rightarrow> ((bool vec \<times> bool vec \<Rightarrow> bool)) \<Rightarrow> (nat set * nat set) set"
+  where "simplicial_complex_induced_by_monotone_boolean_function_ast n f =
+        {z. \<exists>x y. dim_vec x = fst n \<and> dim_vec y = snd n \<and> f (x, y) \<and> ((ceros_of_boolean_input x), (ceros_of_boolean_input y)) = z}"
 
 lemma fst_es_simplice:
-  "a \<in> simplicial_complex_induced_by_monotone_boolean_function_ast f 
-\<Longrightarrow> (\<exists>x y. f x y \<and> (ceros_of_boolean_input x) = fst(a))"
+  "a \<in> simplicial_complex_induced_by_monotone_boolean_function_ast n f
+    \<Longrightarrow> (\<exists>x y. f (x, y) \<and> (ceros_of_boolean_input x) = fst(a))"
   by (smt (verit) fst_conv mem_Collect_eq simplicial_complex_induced_by_monotone_boolean_function_ast_def)
 
 lemma snd_es_simplice:
-  "a \<in> simplicial_complex_induced_by_monotone_boolean_function_ast f 
-\<Longrightarrow> (\<exists>x y. f x y \<and> (ceros_of_boolean_input y) = snd(a))"
+  "a \<in> simplicial_complex_induced_by_monotone_boolean_function_ast n f 
+    \<Longrightarrow> (\<exists>x y. f (x, y) \<and> (ceros_of_boolean_input y) = snd(a))"
   by (smt (verit) snd_conv mem_Collect_eq simplicial_complex_induced_by_monotone_boolean_function_ast_def)
 
-definition set_ast :: "('a set) \<Rightarrow> ('b set) \<Rightarrow> (('a*'b) set)"
+definition set_ast :: "(nat set) set \<Rightarrow> (nat set) set \<Rightarrow> ((nat set*nat set) set)"
   where "set_ast A B \<equiv> {c. \<exists>a\<in>A. \<exists>b\<in>B. c = (a,b)}"
 
-definition set_fst :: "('a::class_mod_type*'b::class_mod_type) set \<Rightarrow> 'a set"
+(*definition set_ast :: "(nat set) \<Rightarrow> (nat set) \<Rightarrow> ((nat*nat) set)"
+  where "set_ast A B \<equiv> {c. \<exists>a\<in>A. \<exists>b\<in>B. c = (a,b)}"*)
+
+definition set_fst :: "(nat*nat) set \<Rightarrow> nat set"
   where "set_fst AB = {a. \<exists>ab\<in>AB. a = fst ab}"
 
 value "set_fst {a, b}"
@@ -43,7 +157,7 @@ proof
     by (smt (verit) SigmaE mem_Collect_eq prod.sel(1) set_fst_def subsetI)
   show "x \<subseteq> set_fst (x \<times> y)"
   proof
-    fix a::"'b"
+    fix a::"nat"
     assume "a \<in> x"
     then obtain b where "b \<in> y" and "(a,b) \<in> (x\<times>y)"
       using assms by blast
@@ -52,134 +166,95 @@ proof
   qed
 qed
 
-definition set_snd :: "('a*'b) set \<Rightarrow> 'b set"
+definition set_snd :: "(nat*nat) set \<Rightarrow> nat set"
   where "set_snd AB = {b. \<exists>ab\<in>AB. b = snd(ab)}"
 
-definition bool_fun_times :: "(bool^('n::class_mod_type) \<Rightarrow> bool) \<Rightarrow> (bool^('m::class_mod_type) \<Rightarrow> bool) \<Rightarrow> (bool^('n*'m) \<Rightarrow> bool)"
-  where "(bool_fun_times f g) x \<equiv>
-     f (bool_vec_from_simplice (set_fst (ceros_of_boolean_input x)))
-   \<and> g (bool_vec_from_simplice (set_snd (ceros_of_boolean_input x)))"
+lemma
+  simplicial_complex_ast_implies_fst_true:
+  assumes "\<gamma> \<in> simplicial_complex_induced_by_monotone_boolean_function_ast nn
+     (bool_fun_ast nn f)"
+  shows "fst f (simplicial_complex.bool_vec_from_simplice (fst nn) (fst \<gamma>))"
+  using assms
+  unfolding simplicial_complex.bool_vec_from_simplice_def
+  unfolding simplicial_complex_induced_by_monotone_boolean_function_ast_def
+  unfolding bool_fun_ast_def
+  unfolding ceros_of_boolean_input_def
+  apply auto
+  by (smt (verit, ccfv_threshold) bool_fun_ast_def case_prod_conv dim_vec index_vec vec_eq_iff)
 
-(* La siguiente condición causa que el teorema pertinente sea incorrecto:
- \<and> (\<nexists>c. \<exists>d\<in>(ceros_of_boolean_input x). c\<in>(ceros_of_boolean_input x) \<and> (fst c < fst d) \<and> (snd c > snd d))*)
+lemma
+  simplicial_complex_ast_implies_snd_true:
+  assumes "\<gamma> \<in> simplicial_complex_induced_by_monotone_boolean_function_ast nn
+     (bool_fun_ast nn f)"
+  shows "snd f (simplicial_complex.bool_vec_from_simplice (snd nn) (snd \<gamma>))"
+  using assms
+  unfolding simplicial_complex.bool_vec_from_simplice_def
+  unfolding simplicial_complex_induced_by_monotone_boolean_function_ast_def
+  unfolding bool_fun_ast_def
+  unfolding ceros_of_boolean_input_def
+  apply auto
+  by (smt (verit, ccfv_threshold) bool_fun_ast_def case_prod_conv dim_vec index_vec vec_eq_iff)
 
-definition
-  simplicial_complex_induced_by_monotone_boolean_function_times 
-    :: "(bool^('n::class_mod_type*'m::class_mod_type) \<Rightarrow> bool) => (('n set)*('m set)) set"
-  where "simplicial_complex_induced_by_monotone_boolean_function_times f = 
-        {z. \<exists>x y. f (bool_vec_from_simplice (x \<times> y)) \<and> (x, y) = z}"
-
-lemma simp_ceros [simp]: "ceros_of_boolean_input (bool_vec_from_simplice (x \<times> y)) = x \<times> y"
-  unfolding bool_vec_from_simplice_def
-  unfolding ceros_of_boolean_input_def by auto
-
-lemma eq_union_or: 
-"simplicial_complex_induced_by_monotone_boolean_function (bool_fun_or f g)
-= simplicial_complex_induced_by_monotone_boolean_function f \<union> simplicial_complex_induced_by_monotone_boolean_function g"
+lemma eq_ast:
+"simplicial_complex_induced_by_monotone_boolean_function_ast (n, m) (bool_fun_ast (n, m) f)
+= set_ast (simplicial_complex_induced_by_monotone_boolean_function n (fst f)) (simplicial_complex_induced_by_monotone_boolean_function m (snd f))"
 proof
-  show "simplicial_complex_induced_by_monotone_boolean_function f \<union> simplicial_complex_induced_by_monotone_boolean_function g \<subseteq> simplicial_complex_induced_by_monotone_boolean_function (bool_fun_or f g)"
+  show "set_ast (simplicial_complex_induced_by_monotone_boolean_function n (fst f))
+     (simplicial_complex_induced_by_monotone_boolean_function m (snd f))
+    \<subseteq> simplicial_complex_induced_by_monotone_boolean_function_ast (n, m)
+        (bool_fun_ast (n, m) f)"
   proof
-    fix \<sigma>::"'a set"
-    assume "\<sigma> \<in> simplicial_complex_induced_by_monotone_boolean_function f \<union> simplicial_complex_induced_by_monotone_boolean_function g"
-    hence "\<sigma> \<in> simplicial_complex_induced_by_monotone_boolean_function f \<or> \<sigma> \<in> simplicial_complex_induced_by_monotone_boolean_function g"
-      by auto
-    hence "f (bool_vec_from_simplice \<sigma>) \<or> g (bool_vec_from_simplice \<sigma>)"
-      by (metis (mono_tags, lifting) bool_vec_set_from_simplice_set_def boolean_function_from_simplicial_complex_def boolean_function_from_simplicial_complex_simplicial_complex_induced_by_monotone_boolean_function_id mem_Collect_eq)
-    hence "bool_fun_or f g (bool_vec_from_simplice \<sigma>)"
-      unfolding bool_fun_or_def
-      by auto
-    thus "\<sigma> \<in> simplicial_complex_induced_by_monotone_boolean_function (bool_fun_or f g)"
-      using simplicial_complex_induced_by_monotone_boolean_function_def
-      by fastforce
-  qed
-next
-  show "simplicial_complex_induced_by_monotone_boolean_function (bool_fun_or f g) \<subseteq> simplicial_complex_induced_by_monotone_boolean_function f \<union> simplicial_complex_induced_by_monotone_boolean_function g"
-  proof
-    fix \<sigma>::"'a set"
-    assume sigma: "\<sigma> \<in> simplicial_complex_induced_by_monotone_boolean_function (bool_fun_or f g)"
-    hence "bool_fun_or f g (bool_vec_from_simplice \<sigma>)"
-      by (metis (mono_tags, lifting) bool_vec_set_from_simplice_set_def boolean_function_from_simplicial_complex_def boolean_function_from_simplicial_complex_simplicial_complex_induced_by_monotone_boolean_function_id mem_Collect_eq)
-    hence "(f (bool_vec_from_simplice \<sigma>)) \<or> (g (bool_vec_from_simplice \<sigma>))"
-      unfolding bool_fun_or_def
-      by auto
-    hence "\<sigma> \<in> simplicial_complex_induced_by_monotone_boolean_function f \<or> \<sigma> \<in> simplicial_complex_induced_by_monotone_boolean_function g"
-      by (smt (z3) sigma bool_fun_or_def mem_Collect_eq simplicial_complex_induced_by_monotone_boolean_function_def)
-    thus "\<sigma> \<in> simplicial_complex_induced_by_monotone_boolean_function f \<union> simplicial_complex_induced_by_monotone_boolean_function g"
-      by auto
-  qed
-qed
-
-lemma eq_inter_and: 
-"simplicial_complex_induced_by_monotone_boolean_function (bool_fun_and f g)
-= simplicial_complex_induced_by_monotone_boolean_function f \<inter> simplicial_complex_induced_by_monotone_boolean_function g"
-proof
-  show "simplicial_complex_induced_by_monotone_boolean_function f \<inter> simplicial_complex_induced_by_monotone_boolean_function g \<subseteq> simplicial_complex_induced_by_monotone_boolean_function (bool_fun_and f g)"
-  proof
-    fix \<sigma>::"'a set"
-    assume "\<sigma> \<in> simplicial_complex_induced_by_monotone_boolean_function f \<inter> simplicial_complex_induced_by_monotone_boolean_function g"
-    hence "\<sigma> \<in> simplicial_complex_induced_by_monotone_boolean_function f \<and> \<sigma> \<in> simplicial_complex_induced_by_monotone_boolean_function g"
-      by auto
-    hence "f (bool_vec_from_simplice \<sigma>) \<and> g (bool_vec_from_simplice \<sigma>)"
-      by (metis (mono_tags, lifting) bool_vec_set_from_simplice_set_def boolean_function_from_simplicial_complex_def boolean_function_from_simplicial_complex_simplicial_complex_induced_by_monotone_boolean_function_id mem_Collect_eq)
-    hence "bool_fun_and f g (bool_vec_from_simplice \<sigma>)"
-      unfolding bool_fun_and_def
-      by auto
-    thus "\<sigma> \<in> simplicial_complex_induced_by_monotone_boolean_function (bool_fun_and f g)"
-      using simplicial_complex_induced_by_monotone_boolean_function_def
-      by fastforce
-  qed
-next
-  show "simplicial_complex_induced_by_monotone_boolean_function (bool_fun_and f g) \<subseteq> simplicial_complex_induced_by_monotone_boolean_function f \<inter> simplicial_complex_induced_by_monotone_boolean_function g"
-  proof
-    fix \<sigma>::"'a set"
-    assume sigma: "\<sigma> \<in> simplicial_complex_induced_by_monotone_boolean_function (bool_fun_and f g)"
-    hence "bool_fun_and f g (bool_vec_from_simplice \<sigma>)"
-      by (metis (mono_tags, lifting) bool_vec_set_from_simplice_set_def boolean_function_from_simplicial_complex_def boolean_function_from_simplicial_complex_simplicial_complex_induced_by_monotone_boolean_function_id mem_Collect_eq)
-    hence "(f (bool_vec_from_simplice \<sigma>)) \<and> (g (bool_vec_from_simplice \<sigma>))"
-      unfolding bool_fun_and_def
-      by auto
-    hence "\<sigma> \<in> simplicial_complex_induced_by_monotone_boolean_function f \<and> \<sigma> \<in> simplicial_complex_induced_by_monotone_boolean_function g"
-      by (smt (z3) sigma bool_fun_and_def mem_Collect_eq simplicial_complex_induced_by_monotone_boolean_function_def)
-    thus "\<sigma> \<in> simplicial_complex_induced_by_monotone_boolean_function f \<inter> simplicial_complex_induced_by_monotone_boolean_function g"
-      by auto
-  qed
-qed
-
-lemma eq_ast: 
-"simplicial_complex_induced_by_monotone_boolean_function_ast (bool_fun_ast f g)
-= set_ast (simplicial_complex_induced_by_monotone_boolean_function f) (simplicial_complex_induced_by_monotone_boolean_function g)"
-proof
-  show "set_ast (simplicial_complex_induced_by_monotone_boolean_function f) (simplicial_complex_induced_by_monotone_boolean_function g) \<subseteq> simplicial_complex_induced_by_monotone_boolean_function_ast (bool_fun_ast f g)"
-  proof
-    fix \<gamma>::"'a set*'b set"
-    assume pert: "\<gamma> \<in> set_ast (simplicial_complex_induced_by_monotone_boolean_function f) (simplicial_complex_induced_by_monotone_boolean_function g)"
-    hence "(fst \<gamma>) \<in> simplicial_complex_induced_by_monotone_boolean_function f"
+    fix \<gamma>::"nat set*nat set"
+    assume pert: "\<gamma> \<in> set_ast (simplicial_complex_induced_by_monotone_boolean_function n (fst f))
+     (simplicial_complex_induced_by_monotone_boolean_function m (snd f))"
+    hence f: "(fst \<gamma>) \<in> simplicial_complex_induced_by_monotone_boolean_function n (fst f)"
       unfolding set_ast_def
       by auto
-    hence sigma: "f (bool_vec_from_simplice (fst \<gamma>))"
-      by (metis (mono_tags, lifting) bool_vec_set_from_simplice_set_def boolean_function_from_simplicial_complex_def boolean_function_from_simplicial_complex_simplicial_complex_induced_by_monotone_boolean_function_id mem_Collect_eq)
-    from pert have "(snd \<gamma>) \<in> simplicial_complex_induced_by_monotone_boolean_function g"
-      unfolding set_ast_def
-      by auto
-    hence tau: "g (bool_vec_from_simplice (snd \<gamma>))"
-      by (metis (mono_tags, lifting) bool_vec_set_from_simplice_set_def boolean_function_from_simplicial_complex_def boolean_function_from_simplicial_complex_simplicial_complex_induced_by_monotone_boolean_function_id mem_Collect_eq)
-    from sigma and tau have sigtau: "bool_fun_ast f g (bool_vec_from_simplice (fst \<gamma>)) (bool_vec_from_simplice (snd \<gamma>))"
+    have sigma: "fst f (simplicial_complex.bool_vec_from_simplice n (fst \<gamma>))"
+      using simplicial_complex.simplicial_complex_implies_true [OF f] .
+    from pert have g: "(snd \<gamma>) \<in> simplicial_complex_induced_by_monotone_boolean_function m (snd f)"
+      unfolding set_ast_def by auto
+    have tau: "(snd f) (simplicial_complex.bool_vec_from_simplice m (snd \<gamma>))"
+      using simplicial_complex.simplicial_complex_implies_true [OF g] .
+    from sigma and tau have sigtau: "bool_fun_ast (n, m) f ((simplicial_complex.bool_vec_from_simplice n (fst \<gamma>)), (simplicial_complex.bool_vec_from_simplice m (snd \<gamma>)))"
       unfolding bool_fun_ast_def
       by auto
-    from sigtau show "\<gamma> \<in> simplicial_complex_induced_by_monotone_boolean_function_ast (bool_fun_ast f g)"
-      using bool_vec_from_simplice_def ceros_of_boolean_input_in_set mem_Collect_eq simplicial_complex_induced_by_monotone_boolean_function_ast_def
-      by fastforce
+    from sigtau show "\<gamma> \<in> simplicial_complex_induced_by_monotone_boolean_function_ast (n, m) (bool_fun_ast (n, m) f)"
+      unfolding simplicial_complex_induced_by_monotone_boolean_function_ast_def
+      unfolding bool_fun_ast_def
+      using sigma apply auto
+      using f g simplicial_complex_induced_by_monotone_boolean_function_def by fastforce
   qed
 next
-  show "simplicial_complex_induced_by_monotone_boolean_function_ast (bool_fun_ast f g) \<subseteq> set_ast (simplicial_complex_induced_by_monotone_boolean_function f) (simplicial_complex_induced_by_monotone_boolean_function g)"
-  proof
-    fix \<gamma>::"'a set*'b set"
-    assume pert: "\<gamma> \<in> simplicial_complex_induced_by_monotone_boolean_function_ast (bool_fun_ast f g)"
-    hence sigma: "(fst \<gamma>) \<in> simplicial_complex_induced_by_monotone_boolean_function f"
-      by (smt (verit) bool_fun_ast_def fst_es_simplice mem_Collect_eq simplicial_complex_induced_by_monotone_boolean_function_def)
-    from pert have tau: "(snd \<gamma>) \<in> simplicial_complex_induced_by_monotone_boolean_function g"
-      by (smt (verit) bool_fun_ast_def snd_es_simplice mem_Collect_eq simplicial_complex_induced_by_monotone_boolean_function_def)
-    from sigma and tau show "\<gamma> \<in> set_ast (simplicial_complex_induced_by_monotone_boolean_function f) (simplicial_complex_induced_by_monotone_boolean_function g)"
+  show "simplicial_complex_induced_by_monotone_boolean_function_ast (n, m)
+     (bool_fun_ast (n, m) f)
+    \<subseteq> set_ast (simplicial_complex_induced_by_monotone_boolean_function n (fst f))
+        (simplicial_complex_induced_by_monotone_boolean_function m (snd f))"
+    proof
+    fix \<gamma>::"nat set*nat set"
+    assume pert: "\<gamma> \<in> simplicial_complex_induced_by_monotone_boolean_function_ast (n, m)
+     (bool_fun_ast (n, m) f)"
+    have sigma: "(fst \<gamma>) \<in> simplicial_complex_induced_by_monotone_boolean_function n (fst f)"
+      unfolding bool_fun_ast_def
+      unfolding simplicial_complex_induced_by_monotone_boolean_function_def
+      unfolding simplicial_complex_induced_by_monotone_boolean_function_ast_def
+      apply auto
+      apply (rule exI [of _ "simplicial_complex.bool_vec_from_simplice n (fst \<gamma>)"], safe)
+      using simplicial_complex.bool_vec_from_simplice_def apply auto[1]
+        apply (metis fst_conv pert simplicial_complex_ast_implies_fst_true)
+      using ceros_of_boolean_input_def simplicial_complex.bool_vec_from_simplice_def apply fastforce
+      using ceros_of_boolean_input_def pert simplicial_complex.bool_vec_from_simplice_def simplicial_complex_induced_by_monotone_boolean_function_ast_def by force
+   have tau: "(snd \<gamma>) \<in> simplicial_complex_induced_by_monotone_boolean_function m (snd f)"
+      unfolding bool_fun_ast_def
+      unfolding simplicial_complex_induced_by_monotone_boolean_function_def
+      unfolding simplicial_complex_induced_by_monotone_boolean_function_ast_def
+      apply auto
+      apply (rule exI [of _ "simplicial_complex.bool_vec_from_simplice m (snd \<gamma>)"], safe)
+      using simplicial_complex.bool_vec_from_simplice_def apply auto[1]
+        apply (metis snd_conv pert simplicial_complex_ast_implies_snd_true)
+      using ceros_of_boolean_input_def simplicial_complex.bool_vec_from_simplice_def apply fastforce
+      using ceros_of_boolean_input_def pert simplicial_complex.bool_vec_from_simplice_def simplicial_complex_induced_by_monotone_boolean_function_ast_def by force
+    from sigma and tau show "\<gamma> \<in> set_ast (simplicial_complex_induced_by_monotone_boolean_function n (fst f)) (simplicial_complex_induced_by_monotone_boolean_function m (snd f))"
       using set_ast_def
       by force
   qed
